Replaced Isabelle's unification with custom one (work in progress), which can include some rewriting; Further examples and experiments.

tests/Old_ZF_Experiments/ZF_Typing_Examples.thy
@@ -23,6 +23,9 @@ lemma set_typeI: "x \<in> A \<Longrightarrow> x ::: set A"
 lemma set_typeE: "x ::: set A \<Longrightarrow> x \<in> A"
   unfolding set_def has_type_Type .
 
+lemma set_type_iff: "(x ::: set A) == Trueprop (x \<in> A)"
+  unfolding set_def has_type_Type .
+
 
 subsection \<open> Type of object-level propositions \<close>
 
@@ -33,11 +36,20 @@ lemma o_TypeI: "(P::o) ::: o"
   unfolding o_def has_type_Type .
 
 
+subsection \<open> Type of subsets of a given set \<close>
+
+abbreviation subset :: "i \<Rightarrow> i type"
+  where "subset A == set (Pow A)"
+
+
+
 subsection \<open> Type declarations for basic material \<close>
 
-lemma eq[type]: "((=)::(i \<Rightarrow> i \<Rightarrow> o)) ::: (x: A) \<Rightarrow> (y: A) \<Rightarrow> o"
+lemma eq_type[type]: "((=)::(i \<Rightarrow> i \<Rightarrow> o)) ::: (x: A) \<Rightarrow> (y: A) \<Rightarrow> o"
   by (intro Pi_typeI o_TypeI)
 
+lemma iff_type[type]: "((\<longleftrightarrow>)::(o \<Rightarrow> o \<Rightarrow> o)) ::: (x: o) \<Rightarrow> (y: o) \<Rightarrow> o"
+  by (intro Pi_typeI o_TypeI)
 
 
 text \<open> Example: Inferring types for list append \<close>
@@ -52,6 +64,7 @@ context
     and [type]: "append ::: (A: Set) \<Rightarrow> (xs: set (List A)) \<Rightarrow> (ys : set (List A)) \<Rightarrow> set (List A)"
 begin
 
+
 ML \<open>Soft_Type_Inference.print_inferred_types @{context} [
   @{term "Nil A = B"}
 ]\<close>
@@ -61,14 +74,38 @@ ML \<open>Soft_Type_Inference.print_inferred_types @{context} [
 ]\<close>
 
 ML \<open>Soft_Type_Inference.print_inferred_types @{context} [
-  @{term "%A x xs. Cons A x xs"}
+  @{term "%A x xs. Cons A x xs = Cons A x xs"}
 ]\<close>
+
+ML \<open>
+
+fun should_throw (P : exn -> unit) (f: unit -> 'a) =
+  case Exn.capture f () of
+    Exn.Exn exn => (P exn
+                    handle Match => error ("Not the expected exception: " ^ @{make_string} exn))
+  | Exn.Res _ => error "Expected exception"                 
+
+\<close>
+
+ML \<open>
+  (fn _ => Soft_Type_Inference.print_inferred_types @{context} [
+     @{term "%A x. Cons A x xs = Cons A x xs"} ])
+  |> should_throw (fn ERROR "Unsolvalbe bound variable in equation." => ())
+\<close>
 
 ML \<open>
 
 Soft_Type_Inference.print_inferred_types @{context} [
   @{term "append A (Cons A x xs) ys = Cons A x (append A xs ys)"},
   @{term "append A (Nil A) ys = ys"} 
+]
+\<close>
+
+ML \<open>
+
+Soft_Type_Inference.print_inferred_types @{context} [
+  @{term_pattern "append _ (Cons _ x xs) ys = Cons _ x (append _ xs ys)"},
+  @{term_pattern "append _ (Nil _) ys = ys"} 
 ]
 \<close>
 
@@ -109,19 +146,63 @@ context
     and [type_simp]: "add (succ n) m = succ (add n m)"
 begin
 
-  
-
-
 
 
 
 ML \<open> Soft_Type_Inference.print_inferred_types @{context} [
-  @{term "vappend A (succ n) m (VCons A n x xs) ys
-   = VCons A (add n m) x (vappend A n m xs ys)"}
+  @{term_pattern "vappend _ _ _ (VCons _ _ x xs) ys
+   = VCons _ _ x (vappend _ _ _ xs ys)"}
 ]\<close>
 
 
 
 end
+
+text \<open> Relations examples \<close>
+
+
+
+
+
+lemma trans_type[type]: "trans ::: (r : set (A * A)) \<Rightarrow> o"
+  by (rule Pi_typeI, rule o_TypeI)
+
+
+lemma All_type[type]: "First_Order_Logic.All ::: (P: ((x::i): A) \<Rightarrow> o) \<Rightarrow> o"
+  by (rule Pi_typeI, rule o_TypeI)
+
+lemma imp_type[type]: "(\<longrightarrow>) ::: (l: o) \<Rightarrow> (r: o) \<Rightarrow> o"
+  by (intro Pi_typeI o_TypeI)
+
+lemma mem_type[type]: "(\<in>) ::: (x: set A) \<Rightarrow> (S: subset A) \<Rightarrow> o"
+  by (intro Pi_typeI o_TypeI)
+
+lemma Pair_type[type]: "Pair ::: (x: set A) \<Rightarrow> (y: set (B x)) \<Rightarrow> set (Sigma A B)"
+proof (intro Pi_typeI)
+  fix x y assume x: "x ::: set A" and y: "y ::: set (B x)"
+  from x have "x \<in> A" by (rule set_typeE)
+  moreover from y have "y \<in> B x" by (rule set_typeE)
+  ultimately have "<x, y> \<in> Sigma A B" by (rule SigmaI)
+  then show "<x, y> ::: set (Sigma A B)" by (rule set_typeI)
+qed
+
+context
+
+begin
+
+
+ML \<open> Soft_Type_Context.get (Context.Proof @{context}) \<close>
+
+(*
+ML \<open> Soft_Type_Inference.print_inferred_types @{context} [
+  @{term "\<forall>x y z. <x,y>: r \<longrightarrow> <y,z>: r \<longrightarrow> <x,z>: r"}
+]\<close>
+*)
+
+
+
+end
+
+
 
 end
